examples/arm6/evaluate/arm_rulesLib.sig
@@ -1,0 +1,8 @@
+signature arm_rulesLib =
+sig
+    include Abbrev
+
+    val SORT_REG_WRITEL_CONV : conv
+    val REG_READ_WRITEL_CONV : conv
+    val REG_WRITEL_CONV      : conv
+end
