examples/arm6/evaluate/arm_rulesLib.sml
@@ -1,0 +1,85 @@
+(* ========================================================================= *)
+(* FILE          : arm_rulesLib.sml                                          *)
+(* DESCRIPTION   : Tools for symbolic evaluation of the ARM Instruction Set  *)
+(*                                                                           *)
+(* AUTHORS       : (c) Anthony Fox, University of Cambridge                  *)
+(* DATE          : 2006                                                      *)
+(* ========================================================================= *)
+
+structure arm_rulesLib :> arm_rulesLib =
+struct
+
+(* interactive use:
+  app load ["arm_rulesTheory"];
+*)
+
+open HolKernel boolLib Parse bossLib;
+open Q wordsTheory arm_rulesTheory;
+
+(* ------------------------------------------------------------------------- *)
+
+val wrd_ss = std_ss ++ rewrites [dimindex_4,word_ls_n2w,n2w_11];
+
+val REG_WRITE_WRITE_PC = (GEN_ALL o GSYM o SIMP_RULE std_ss [] o
+  INST [`m1` |-> `usr`,`m2` |-> `m`] o DISCH `~(n = 15w)` o
+  SPEC_ALL) lemmasTheory.REG_WRITE_WRITE_PC;
+
+val REG_WRITE_WRITE_PC2 = (GEN_ALL o SIMP_RULE std_ss [] o
+  INST [`n` |-> `15w`] o SPEC_ALL) lemmasTheory.REG_WRITE_WRITE_PC;
+
+val REG_WRITEL_PC = GEN_ALL
+ ((SIMP_CONV std_ss [REG_WRITEL_def,lemmasTheory.TO_WRITE_READ6] THENC
+   REWRITE_CONV [REG_WRITE_WRITEL]) ``REG_WRITEL r m [(15w,d)]``);
+
+val REG_WRITEL_WRITEL_PC = (GEN_ALL o ONCE_REWRITE_RULE [REG_WRITEL_PC] o
+  INST [`l1` |-> `[(15w,d)]`] o SPEC_ALL) REG_WRITEL_WRITEL;
+
+val SORT_REG_WRITEL_CONV =
+  SIMP_CONV wrd_ss [INC_PC,REG_READ_WRITEL_PC2] THENC
+  SIMP_CONV wrd_ss [REG_WRITEL_def,REG_WRITE_WRITE_THM,
+    REG_WRITE_WRITE_PC,REG_WRITE_WRITE_PC2] THENC
+  REWRITE_CONV [listTheory.APPEND,REG_WRITE_WRITEL,
+    REG_WRITEL_WRITEL,REG_WRITEL_WRITEL_PC];
+
+val REG_READ_WRITEL_CONV = SIMP_CONV std_ss
+    [CONJUNCT1 REG_WRITEL_def,REG_READ_WRITEL,REG_READ_WRITEL_PC,
+     REG_READ_WRITEL_PC2,dimindex_4,n2w_11];
+
+val REG_WRITEL_CONV = SORT_REG_WRITEL_CONV THENC REG_READ_WRITEL_CONV;
+
+(* ------------------------------------------------------------------------- *)
+
+fun mk_abbrev v  = mk_comb(``Abbrev``,mk_eq(v,genvar (type_of v)));
+
+val dest_abbrev = dest_eq o snd o dest_comb;
+
+fun is_abbrev_match m t =
+let val v = fst (dest_abbrev m)
+    val rrl = match_term m t
+in
+  null (snd rrl) andalso
+  not (isSome (List.find (fn x => term_eq (#redex x) v) (fst rrl)))
+end;
+
+fun total_is_abbrev_match m t =
+  case total (is_abbrev_match m) t of
+    SOME b => b
+  | _ => false;
+    
+fun get_abbrev_match m t = find_term (total_is_abbrev_match m) t;
+
+fun UNABBREV_RULE q thm =
+let val t = concl thm
+    val m = mk_abbrev (parse_in_context (free_vars t) q)
+    val mt = get_abbrev_match m t
+    val (l,r) = dest_abbrev mt
+in
+  SIMP_RULE bool_ss [SPEC `T` markerTheory.Abbrev_def] (Thm.INST [l |-> r] thm)
+end;
+
+fun UNABBREVL_RULE l t =
+   GEN_ALL (foldl (fn (x,t) => UNABBREV_RULE x t) (SPEC_ALL t) l);
+
+(* ------------------------------------------------------------------------- *)
+
+end
